S4 with progress and preservation, modulo a substitution lemma.

S4/S4.v
@@ -162,7 +162,7 @@ Inductive value : tm -> Prop :=
 
 Reserved Notation "'[' x ':=' s ']' t" (in custom stlc_tm at level 20, x constr).
 
-Fixpoint subst (x : string) (s : tm) (t : tm) : tm :=
+Fixpoint local_subst (x : string) (s : tm) (t : tm) : tm :=
   match t with
   | tm_var y =>
       if x =? y then s else t
@@ -180,7 +180,7 @@ Fixpoint subst (x : string) (s : tm) (t : tm) : tm :=
 
   (* Box operators *)
   | <{ box t }> =>
-      <{ box ([x := s] t) }>
+      <{ box t }>
   | <{ unbox y := t1 in t2 }> =>
       if x =? y then <{ unbox y := [x := s] t1 in t2 }>
       else <{ unbox y := [x := s] t1 in [x := s] t2 }>
@@ -188,19 +188,57 @@ Fixpoint subst (x : string) (s : tm) (t : tm) : tm :=
   | <{ dia t }> =>
       <{ dia ([x := s] t) }>
   | <{ undia y := t1 in t2 }> =>
-      <{ undia y := [x := s] t1 in t2 }>
+      if x =? y then <{ undia y := [x := s] t1 in t2 }>
+      else <{ undia y := [x := s] t1 in [x := s] t2 }>
   end
 
-where "'[' x ':=' s ']' t" := (subst x s t) (in custom stlc_tm).
+where "'[' x ':=' s ']' t" := (local_subst x s t) (in custom stlc_tm).
+
+
+Reserved Notation "'[[' x ':=' s ']]' t" (in custom stlc_tm at level 20, x constr).
+
+Fixpoint global_subst (x : string) (s : tm) (t : tm) : tm :=
+  match t with
+  | tm_var y =>
+      if x =? y then s else t
+  | <{\y : T , t1}> =>
+      if x =? y then t else <{\y : T, [[x:=s]] t1}>
+  | <{t1 t2}> =>
+    <{([[x:=s]] t1) ([[x:=s]] t2)}>
+  (* Booleans *)
+  | <{ true }>  =>
+      <{ true }>
+  | <{ false }> =>
+      <{ false }>
+  | <{if t1 then t2 else t3}> =>
+      <{if ([[x:=s]] t1) then ([[x:=s]] t2) else ([[x:=s]] t3)}>
+
+  (* Box operators *)
+  | <{ box t }> =>
+      <{ box [[x:=s]] t }>
+  | <{ unbox y := t1 in t2 }> =>
+      if x =? y then <{ unbox y := [[x := s]] t1 in t2 }>
+      else <{ unbox y := [[x := s]] t1 in [[x := s]] t2 }>
+  (* Diamond operators *)
+  | <{ dia t }> =>
+      <{ dia ([[x := s]] t) }>
+  | <{ undia y := t1 in t2 }> =>
+      if x =? y then <{ undia y := [[x := s]] t1 in t2 }>
+      else <{ undia y := [[x := s]] t1 in [[x := s]] t2 }>
+  end
+
+where "'[[' x ':=' s ']]' t" := (global_subst x s t) (in custom stlc_tm).
 
 Reserved Notation "'〈' x ':=' s '〉' t" (in custom stlc_tm at level 20, x constr).
 
 (* This is not the right name... *)
 Fixpoint delay (x : string) (s : tm) (t : tm) : tm :=
-  match t with
+  match s with
   | <{ undia y := t1 in t2 }> =>
-      <{ undia y := t1 in 〈x := s〉 t2 }>
-  | t => <{[x := s]t}>
+      <{ undia y := t1 in 〈x := t2〉 t }>
+  | <{ unbox y := t1 in t2 }> =>
+      <{ unbox y := t1 in 〈x := t2〉 t }>
+  | s' => <{[x := s']t}>
   end
 
 where "'〈' x ':=' s '〉' t" := (delay x s t) (in custom stlc_tm).
@@ -261,14 +299,22 @@ Inductive step : tm -> tm -> Prop :=
 | ST_Box : forall t1 t1',
     t1 --> t1' ->
     <{ box t1 }> --> <{ box t1' }>
+| ST_Unbox1 : forall x t1 t1' t2,
+    t1 --> t1' ->
+    <{unbox x := t1 in t2}> -->
+    <{unbox x := t1' in t2}>
 | ST_Unbox : forall x t1 t2,
     <{unbox x := box t1 in t2}> -->
-    <{ [x := t1]t2 }>
+    <{ [[x := t1]]t2 }>
 
 (* Diamond Operator *)
 | ST_Dia : forall t1 t1',
     t1 --> t1' ->
     <{ dia t1 }> --> <{ dia t1' }>
+| ST_Undia1 : forall x t1 t1' t2,
+    t1 --> t1' ->
+    <{undia x := t1 in t2}> -->
+    <{undia x := t1' in t2}>
 | ST_Undia : forall x t1 t2,
     <{undia x := dia t1 in t2}> -->
     <{ 〈 x := t1〉t2 }>
@@ -298,20 +344,40 @@ Reserved Notation "Gamma '|-' t '\in' T"
             (at level 101,
              t custom stlc_tm, T custom stlc_ty at level 0).
 
-Definition context := (partial_map ty * partial_map ty)%type.
+Inductive var_scope :=
+| local : ty -> var_scope
+| global : ty -> var_scope.
+
+Definition context := partial_map var_scope.
+
+Definition global_context (Gamma : context) : context :=
+  fun x => match Gamma x with
+           | Some (global T) => Some (global T)
+           | _ => None
+           end.
+
+Lemma global_context_OK :
+  forall Gamma,
+    ((forall x T, Gamma x = Some (global T) -> (global_context Gamma) x = Some (global T)) /\
+       (forall x T, (global_context Gamma) x = Some (global T) -> Gamma x = Some (global T)) /\
+       (forall x T, (global_context Gamma) x <> Some (local T))).
+Proof.
+  unfold global_context; intuition; try rewrite H; eauto.
+  destruct (Gamma x0) as [ [? | ?] | ]; simpl in *; congruence.
+  destruct (Gamma x0) as [ [? | ?] | ]; simpl in *; congruence.
+Qed.
 
 Inductive has_type : context -> tm -> ty -> Prop :=
 (* Lambda Terms *)
-| T_Var1 : forall Delta Gamma x T1,
-    Gamma x = Some T1 ->
-    (Delta, Gamma) |- x \in T1
-
-| T_Var2 : forall Delta Gamma x T1,
-    Delta x = Some T1 ->
-    (Delta, Gamma) |- x \in T1
-| T_Abs : forall Delta Gamma x T1 T2 t1,
-    (Delta, x |-> T2 ; Gamma) |- t1 \in T1 ->
-      (Delta, Gamma) |- \x:T2, t1 \in (T2 -> T1)
+| T_Var1 : forall Gamma x T1,
+    Gamma x = Some (local T1) ->
+    Gamma |- x \in T1
+| T_Var2 : forall Gamma x T1,
+    Gamma x = Some (global T1) ->
+    Gamma |- x \in T1
+| T_Abs : forall Gamma x T1 T2 t1,
+    x |-> local T2 ; Gamma |- t1 \in T1 ->
+      Gamma |- \x:T2, t1 \in (T2 -> T1)
 | T_App : forall T1 T2 Gamma t1 t2,
       Gamma |- t1 \in (T2 -> T1) ->
       Gamma |- t2 \in T2 ->
@@ -329,31 +395,43 @@ Inductive has_type : context -> tm -> ty -> Prop :=
        Gamma |- if t1 then t2 else t3 \in T1
 
 (* Box Operators *)
-| T_Box : forall Delta Gamma t T,
-    (Delta, empty) |- t \in T ->
-    (Delta, Gamma) |- box t \in □T
-| T_Unbox : forall Delta Gamma x t1 t2 T1 T2 ,
-    (Delta, Gamma) |- t1 \in ( □T1 ) ->
-    (x |-> T1; Delta, Gamma) |- t2 \in T2  ->
-    (Delta, Gamma) |- unbox x := t1 in t2 \in T2
+| T_Box : forall Gamma t T,
+    global_context Gamma |- t \in T ->
+    Gamma |- box t \in □T
+| T_Unbox : forall Gamma x t1 t2 T1 T2 ,
+    Gamma |- t1 \in ( □T1 ) ->
+    (x |-> global T1; Gamma) |- t2 \in T2  ->
+    Gamma |- unbox x := t1 in t2 \in T2
 
 (* Dia Operators *)
-| T_Dia : forall Delta Gamma t T,
-    (Delta, Gamma) |- t \in T ->
-    (Delta, Gamma) |- dia t \in ♢T
-| T_Undia : forall Delta Gamma x t1 t2 T1 T2 ,
-    (Delta, Gamma) |- t1 \in ( ♢T1 ) ->
-    (Delta, x |-> T1; Gamma) |- t2 \in T2  ->
-    (Delta, Gamma) |- undia x := t1 in t2 \in T2
+| T_Dia : forall Gamma t T,
+    has_local_type Gamma t T ->
+    Gamma |- dia t \in ♢T
+
+with has_local_type : context -> tm -> ty -> Prop :=
+| LT_Undia : forall Gamma x t1 t2 T1 T2 ,
+    Gamma |- t1 \in ( ♢T1 ) ->
+    has_local_type (x |-> local T1; Gamma) t2 T2  ->
+    has_local_type Gamma <{undia x := t1 in t2}> T2
+| LT_Unbox : forall Gamma x t1 t2 T1 T2 ,
+    Gamma |- t1 \in ( □T1 ) ->
+    has_local_type (x |-> global T1; Gamma) t2 T2  ->
+    has_local_type Gamma <{unbox x := t1 in t2}> T2
+| LT_global : forall Gamma t T,
+    Gamma |- t \in T ->
+    has_local_type Gamma t T
 
 where "Gamma '|-' t '\in' T" := (has_type Gamma t T).
+
+Scheme has_type_ind' := Induction for has_type Sort Prop
+  with has_local_type_ind' := Induction for has_local_type Sort Prop.
 
 (* All our favorite Modal Axioms: *)
 
 (* λx:A ⊃ B ⊃ C. λy:A ⊃ B. λz:A. (x z) (y z)
    : (A ⊃ B ⊃ C) ⊃(A ⊃ B) ⊃ A ⊃ C *)
 Example Modal_Axiom_1 : forall A B C,
-   (empty, empty) |- \x:A -> B -> C, \y:A -> B, \z:A, (x z) (y z)
+   empty |- \x:A -> B -> C, \y:A -> B, \z:A, (x z) (y z)
    \in ((A -> B -> C) -> (A -> B) -> A -> C).
 Proof.
   repeat econstructor.
@@ -362,7 +440,7 @@ Qed.
 (* λx:A. λy:B. x
    : A ⊃ B ⊃ A *)
 Example Modal_Axiom_2 : forall A B,
-    (empty, empty) |- \x : A, \y : B, x \in (A -> B -> A).
+    empty |- \x : A, \y : B, x \in (A -> B -> A).
 Proof.
   repeat econstructor.
 Qed.
@@ -370,7 +448,7 @@ Qed.
 (* λx:□(A ⊃ B). λy:□A. let box u = x in let box w = y in box (u w)
    : □(A ⊃ B) ⊃(□A ⊃ □B) *)
 Example Modal_Axiom_3 : forall A B,
-    (empty, empty) |-
+    empty |-
       \x:□(A -> B), \y:□A, (unbox u := x in unbox w := y in box (u w))
         \in ((□(A -> B)) -> (□A) -> (□B)).
 Proof.
@@ -389,7 +467,7 @@ Qed.
 (* λx:□A. let box u = x in u
 : □A ⊃ A *)
 Example Modal_Axiom_4 : forall A,
-    (empty, empty) |- \y : □A, unbox u := y in u \in ((□A) -> A).
+    empty |- \y : □A, unbox u := y in u \in ((□A) -> A).
 Proof.
   econstructor.
   econstructor.
@@ -400,7 +478,7 @@ Qed.
 (* λx:□A. let box u = x in box box u
    : □A ⊃ □□A *)
 Example Modal_Axiom_5 : forall A,
-    (empty, empty) |- \x : □A, unbox u := x in box (box u) \in ((□A) -> (□ (□ A))).
+    empty |- \x : □A, unbox u := x in box (box u) \in ((□A) -> (□ (□ A))).
 Proof.
   econstructor.
   econstructor.
@@ -413,7 +491,7 @@ Qed.
 (* λx:A. dia x
    : A ⊃ ♢A *)
 Example Modal_Axiom_6 : forall A,
-    (empty, empty) |- \x : A, dia x \in (A -> ♢A).
+    empty |- \x : A, dia x \in (A -> ♢A).
 Proof.
   repeat econstructor.
 Qed.
@@ -421,7 +499,7 @@ Qed.
 (* λx:♢♢A. dia (let dia y = x in let dia z = y in z)
    : ♢♢A ⊃ ♢A *)
 Example Modal_Axiom_7 : forall A,
-    (empty, empty) |- \x : ♢♢A, dia (undia y := x in undia z := y in z) \in ((♢♢A) -> ♢A).
+    empty |- \x : ♢♢A, dia (undia y := x in undia z := y in z) \in ((♢♢A) -> ♢A).
 Proof.
   repeat econstructor.
 Qed.
@@ -429,7 +507,7 @@ Qed.
 (* λx:□(A ⊃ B). λy:♢A. let box u = x in dia (let dia z = y in u z)
    : □(A ⊃ B) ⊃(♢A ⊃ ♢B) *)
 Example Modal_Axiom_8 : forall A B,
-    (empty, empty) |- \x : □(A -> B), \y : ♢A, unbox u := x in dia (undia z := y in u z)
+    empty |- \x : □(A -> B), \y : ♢A, unbox u := x in dia (undia z := y in u z)
                                                                    \in ((□(A -> B)) -> (♢A) -> ♢B).
 Proof.
   econstructor.
@@ -440,13 +518,14 @@ Proof.
     econstructor.
     + repeat econstructor.
     + econstructor.
+      econstructor.
       * econstructor 2; reflexivity.
       * repeat econstructor.
 Qed.
 
 Example quote_is_typed (A : ty) :
   let t := quote A in
-  (empty, empty) |- t \in ((□A) -> (□□A)).
+  empty |- t \in ((□A) -> (□□A)).
 Proof.
   econstructor.
   econstructor.
@@ -458,7 +537,7 @@ Qed.
 
 Example apply_is_typed (A B : ty) :
   let t := apply A B in
-  (empty, empty) |- t \in ((□A -> B) -> (□A) -> □B).
+  empty |- t \in ((□A -> B) -> (□A) -> □B).
 Proof.
   econstructor.
   econstructor.
@@ -470,4 +549,445 @@ Proof.
       econstructor.
       econstructor 2; reflexivity.
       econstructor 2; reflexivity.
+Qed.
+
+Hint Constructors has_type.
+
+Lemma canonical_forms_bool : forall t,
+  empty |- t \in Bool ->
+  value t ->
+  (t = <{true}>) \/ (t = <{false}>).
+Proof.
+  intros t HT HVal.
+  destruct HVal; auto; inversion HT.
+Qed.
+
+Lemma canonical_forms_fun : forall t T1 T2,
+  empty |- t \in (T1 -> T2) ->
+  value t ->
+  exists x u, t = <{\x:T1, u}>.
+Proof.
+  intros t T1 T2 HT HVal.
+  destruct HVal; inversion HT; subst; eauto.
+Qed.
+
+Lemma canonical_forms_box : forall t T,
+  empty |- t \in (□ T) ->
+  value t ->
+  exists u, t = <{box u}>.
+Proof.
+  intros t T HT HVal.
+  destruct HVal; auto; inversion HT; subst; eauto.
+Qed.
+
+Lemma canonical_forms_diamond : forall t T,
+  empty |- t \in (♢ T) ->
+  value t ->
+  exists u, t = <{dia u}>.
+Proof.
+  intros t T HT HVal.
+  destruct HVal; auto; inversion HT; subst; eauto.
+Qed.
+
+Theorem progress : forall t T,
+  empty |- t \in T ->
+  value t \/ exists t', t --> t'.
+Proof with eauto.
+  intros t T Ht.
+  remember empty as Gamma.
+  induction Ht; try injection HeqGamma; intros; subst;
+    try discriminate; try solve [left; constructor].
+  - (* T_App *)
+    (* [t] = [t1 t2].  Proceed by cases on whether [t1] is a
+       value or steps... *)
+    right. destruct IHHt1...
+    + (* t1 is a value *)
+      destruct IHHt2...
+      * (* t2 is also a value *)
+        eapply canonical_forms_fun in Ht1; [|assumption].
+        destruct Ht1 as [x [t0 H1] ]. subst.
+        exists (<{ [x:=t2]t0 }>).
+        econstructor; eauto.
+      * (* t2 steps *)
+        destruct H0 as [t2' Hstp]. exists (<{t1 t2'}>).
+        econstructor 3; eauto.
+    + (* t1 steps *)
+      destruct H as [t1' Hstp]. exists (<{t1' t2}>)...
+      econstructor; eauto.
+  - (* T_If *)
+    right. destruct IHHt1...
+
+    + (* t1 is a value *)
+      destruct (canonical_forms_bool t1); subst; eauto.
+      * exists t2; econstructor; eauto.
+      * exists t3; econstructor; eauto.
+    + (* t1 also steps *)
+      destruct H as [t1' Hstp]. exists <{if t1' then t2 else t3}>...
+      econstructor; eauto.
+  - (* T_Box *)
+    right. destruct IHHt1...
+    + (* t1 is a value *)
+      destruct (canonical_forms_box t1 T1); subst; eauto.
+      * eexists; econstructor 9.
+    + destruct H as [t1' Hstp].
+      eexists; econstructor; eauto.
+Qed.
+
+Lemma weakening : forall Gamma Gamma' t T,
+    inclusion Gamma Gamma' ->
+    Gamma  |- t \in T  -> Gamma' |- t \in T.
+Proof.
+  intros Gamma Gamma' t T HInc Ht;
+    revert Gamma' HInc.
+  pattern Gamma, t, T, Ht;
+    eapply has_type_ind' with
+    (P := fun Gamma t T _ => forall Gamma' : partial_map var_scope, inclusion Gamma Gamma' -> Gamma' |- t \in T)
+    (P0 := fun Gamma t T _ => forall Gamma' : partial_map var_scope, inclusion Gamma Gamma' -> has_local_type Gamma' t T); eauto using inclusion_update; clear; intros.
+  - econstructor.
+    eapply H; eauto; compute; eauto.
+    unfold inclusion in H0.
+    intros; specialize (H0 x0 v); destruct (Gamma x0) as [ [? | ?] | ]; try congruence.
+    rewrite H0; injection H1; intros; subst; congruence.
+  - econstructor; eauto.
+    eapply H0; eauto using inclusion_update.
+  - econstructor; eauto using inclusion_update.
+  - econstructor; eauto.
+Qed.
+
+Lemma local_weakening : forall Gamma Gamma' t T,
+    inclusion Gamma Gamma' ->
+    has_local_type Gamma t T  -> has_local_type Gamma' t T.
+Proof.
+  intros Gamma Gamma' t T HInc Ht;
+    revert Gamma' HInc;
+    induction Ht; simpl; intros;
+    econstructor; eauto using weakening, inclusion_update.
+Qed.
+
+Lemma local_substitution_preserves_typing
+  : forall Gamma x U t v T,
+  (x |-> local U; Gamma) |- t \in T ->
+  empty |- v \in U   ->
+  Gamma |- [x:=v]t \in T.
+Proof.
+  intros Gamma x U t v T Ht.
+  remember (x |-> local U; Gamma) as Gamma'.
+  generalize dependent Gamma.
+  pattern Gamma', t, T, Ht;
+    eapply has_type_ind' with
+    (P := fun Gamma' t T _ =>
+            forall
+              (Gamma : partial_map var_scope)
+              (Heq : Gamma' = (x |-> local U; Gamma))
+              (Hv : empty |- v \in U),
+              Gamma |- [x := v] t \in T)
+    (P0 := fun Gamma' t T _ =>
+             forall
+               (Gamma : partial_map var_scope)
+               (Heq : Gamma' = (x |-> local U; Gamma))
+               (Hv : empty |- v \in U),
+               has_local_type Gamma (<{[x := v] t}>) T);
+    eauto using inclusion_update; clear; intros; subst; simpl; eauto.
+  - (* var1 *)
+    rename x0 into y. destruct (eqb_stringP x y); subst.
+    + (* x=y *)
+      rewrite update_eq in e.
+      injection e as H2; subst.
+      rewrite eqb_refl; intros; eapply weakening; try eassumption;
+        unfold inclusion; eauto.
+      compute; congruence.
+    + (* x<>y *)
+      rewrite (proj2 (eqb_neq x y)); eauto.
+      intros; apply T_Var1. rewrite update_neq in e; auto.
+  - rename x0 into y. destruct (eqb_stringP x y); subst.
+    + (* x=y *)
+      rewrite update_eq in e; congruence.
+    + (* x<>y *)
+      rewrite (proj2 (eqb_neq x y)); eauto.
+      intros; apply T_Var2. rewrite update_neq in e; auto.
+  - (* abs *)
+    rename x0 into y.
+    destruct (eqb_stringP x y); subst.
+    + (* x=y *)
+      rewrite eqb_refl.
+      apply T_Abs.
+      rewrite update_shadow in h. assumption.
+    +  (* x<>y *)
+      rewrite (proj2 (eqb_neq x y)); eauto.
+      apply T_Abs.
+      apply H; eauto.
+      rewrite update_permute; auto.
+  - (* box *)
+    econstructor.
+    eapply weakening; try eassumption.
+    unfold inclusion; simpl; intros.
+    unfold update, t_update, global_context in *|-*.
+    destruct (eqb_stringP x x0); subst; eauto.
+    congruence.
+  - rename x0 into y.
+    destruct (eqb_stringP x y); subst.
+    + (* x=y *)
+      rewrite eqb_refl.
+      rewrite update_shadow in h0.
+      econstructor; eauto.
+    +  (* x<>y *)
+      rewrite (proj2 (eqb_neq x y)); eauto.
+      eapply T_Unbox.
+      * apply H; eauto.
+      * eapply H0; eauto.
+        rewrite update_permute; auto.
+  - rename x0 into y.
+    destruct (eqb_stringP x y); subst.
+    + (* x=y *)
+      rewrite eqb_refl.
+      rewrite update_shadow in h0.
+      econstructor; eauto.
+    +  (* x<>y *)
+      rewrite (proj2 (eqb_neq x y)); eauto.
+      eapply LT_Undia.
+      * apply H; eauto.
+      * eapply H0; eauto.
+        rewrite update_permute; auto.
+  - rename x0 into y.
+    destruct (eqb_stringP x y); subst.
+    + (* x=y *)
+      rewrite eqb_refl.
+      rewrite update_shadow in h0.
+      econstructor; eauto.
+    +  (* x<>y *)
+      rewrite (proj2 (eqb_neq x y)); eauto.
+      eapply LT_Unbox.
+      * apply H; eauto.
+      * eapply H0; eauto.
+        rewrite update_permute; auto.
+  - econstructor; eauto.
+Qed.
+
+Theorem local_substitution_preserves_local_typing : forall Gamma x U t v T,
+    has_local_type (x |-> local U; Gamma) t T ->
+    empty |- v \in U   ->
+  has_local_type Gamma <{[x:=v]t}> T.
+Proof.
+  intros Gamma x U t v T Ht.
+  remember (x |-> local U; Gamma) as Gamma'.
+  generalize dependent Gamma.
+  induction Ht; intros; subst; simpl; eauto.
+  - rename x0 into y.
+    destruct (eqb_stringP x y); subst.
+    + (* x=y *)
+      rewrite eqb_refl.
+      rewrite update_shadow in Ht.
+      econstructor; eauto using local_substitution_preserves_typing.
+    +  (* x<>y *)
+      rewrite (proj2 (eqb_neq x y)); eauto.
+      econstructor; eauto using local_substitution_preserves_typing.
+      eapply IHHt; eauto.
+      rewrite update_permute; auto.
+  - rename x0 into y.
+    destruct (eqb_stringP x y); subst.
+    + (* x=y *)
+      rewrite eqb_refl.
+      rewrite update_shadow in Ht.
+      econstructor; eauto using local_substitution_preserves_typing.
+    + rewrite (proj2 (eqb_neq x y)); eauto.
+      econstructor; eauto using local_substitution_preserves_typing.
+      eapply IHHt; eauto.
+      rewrite update_permute; auto.
+  - econstructor; eauto using local_substitution_preserves_typing.
+Qed.
+
+Lemma global_substitution_preserves_typing : forall Gamma x U t v T,
+  (x |-> global U; Gamma) |- t \in T ->
+  empty |- v \in U   ->
+  Gamma |- [[x:=v]]t \in T.
+Proof.
+  intros Gamma x U t v T Ht.
+  remember (x |-> global U; Gamma) as Gamma'.
+  generalize dependent Gamma.
+  pattern Gamma', t, T, Ht;
+    eapply has_type_ind' with
+    (P := fun Gamma' t T _ =>
+            forall
+              (Gamma : partial_map var_scope)
+              (Heq : Gamma' = (x |-> global U; Gamma))
+                   (Hv : empty |- v \in U),
+              Gamma |- [[x := v]] t \in T)
+    (P0 := fun Gamma' t T _ =>
+             forall
+               (HId : has_local_type Gamma' t T)
+               (Gamma : partial_map var_scope)
+                    (Heq : Gamma' = (x |-> global U; Gamma))
+                    (Hv : empty |- v \in U),
+               has_local_type Gamma (<{[[x := v]] t}>) T);
+    eauto using inclusion_update; clear; intros; subst; simpl; eauto.
+  - (* var1 *)
+    rename x0 into y. destruct (eqb_stringP x y); subst.
+    + (* x=y *)
+      rewrite update_eq in e.
+      injection e as H2; subst.
+      rewrite eqb_refl; intros; eapply weakening; try eassumption;
+        unfold inclusion; eauto.
+      compute; discriminate.
+    + (* x<>y *)
+      rewrite (proj2 (eqb_neq x y)); eauto.
+      intros; apply T_Var1. rewrite update_neq in e; auto.
+  - rename x0 into y. destruct (eqb_stringP x y); subst.
+    + (* x=y *)
+      rewrite eqb_refl.
+      rewrite update_eq in e; injection e; intros; subst.
+      eapply weakening; eauto.
+      compute; congruence.
+    + (* x<>y *)
+      rewrite (proj2 (eqb_neq x y)); eauto.
+      intros; apply T_Var2. rewrite update_neq in e; auto.
+  - (* abs *)
+    rename x0 into y.
+    destruct (eqb_stringP x y); subst.
+    + (* x=y *)
+      rewrite eqb_refl.
+      apply T_Abs.
+      rewrite update_shadow in h. assumption.
+    +  (* x<>y *)
+      rewrite (proj2 (eqb_neq x y)); eauto.
+      apply T_Abs.
+      apply H; eauto.
+      rewrite update_permute; auto.
+  - (* box *)
+    econstructor.
+    eapply H; eauto.
+    eapply functional_extensionality; intros.
+    unfold update, t_update, global_context in *|-*.
+    destruct (eqb_stringP x x0); subst; eauto.
+  - rename x0 into y.
+    destruct (eqb_stringP x y); subst.
+    + (* x=y *)
+      rewrite eqb_refl.
+      rewrite update_shadow in h0.
+      econstructor; eauto.
+    +  (* x<>y *)
+      rewrite (proj2 (eqb_neq x y)); eauto.
+      eapply T_Unbox.
+      * apply H; eauto.
+      * eapply H0; eauto.
+        rewrite update_permute; auto.
+  - rename x0 into y.
+    destruct (eqb_stringP x y); subst.
+    + (* x=y *)
+      rewrite eqb_refl.
+      rewrite update_shadow in h0.
+      econstructor; eauto.
+    +  (* x<>y *)
+      rewrite (proj2 (eqb_neq x y)); eauto.
+      eapply LT_Undia.
+      * apply H; eauto.
+      * eapply H0; eauto.
+        rewrite update_permute; auto.
+  - rename x0 into y.
+    destruct (eqb_stringP x y); subst.
+    + (* x=y *)
+      rewrite eqb_refl.
+      rewrite update_shadow in h0.
+      econstructor; eauto.
+    +  (* x<>y *)
+      rewrite (proj2 (eqb_neq x y)); eauto.
+      eapply LT_Unbox.
+      * apply H; eauto.
+      * eapply H0; eauto.
+        rewrite update_permute; auto.
+  - econstructor; eauto.
+Qed.
+
+Theorem global_substitution_preserves_local_typing : forall Gamma x U t v T,
+    has_local_type (x |-> global U; Gamma) t T ->
+  empty |- v \in U   ->
+  has_local_type Gamma <{[[x:=v]]t}> T.
+Proof.
+  intros Gamma x U t v T Ht.
+  remember (x |-> global U; Gamma) as Gamma'.
+  generalize dependent Gamma.
+  induction Ht; intros; subst; simpl; eauto.
+  - rename x0 into y.
+    destruct (eqb_stringP x y); subst.
+    + (* x=y *)
+      rewrite eqb_refl.
+      rewrite update_shadow in Ht.
+      econstructor; eauto using global_substitution_preserves_typing.
+    +  (* x<>y *)
+      rewrite (proj2 (eqb_neq x y)); eauto.
+      econstructor; eauto using global_substitution_preserves_typing.
+      eapply IHHt; eauto.
+      rewrite update_permute; auto.
+  - rename x0 into y.
+    destruct (eqb_stringP x y); subst.
+    + (* x=y *)
+      rewrite eqb_refl.
+      rewrite update_shadow in Ht.
+      econstructor; eauto using global_substitution_preserves_typing.
+    + rewrite (proj2 (eqb_neq x y)); eauto.
+      econstructor; eauto using global_substitution_preserves_typing.
+      eapply IHHt; eauto.
+      rewrite update_permute; auto.
+  - econstructor; eauto using global_substitution_preserves_typing.
+Qed.
+
+Lemma delaying_preserves_local_typing
+  : forall Gamma x U t v T,
+    has_local_type (x |-> local U; Gamma) t T ->
+    has_local_type empty v U   ->
+    has_local_type Gamma <{〈 x := v〉t}> T.
+Proof.
+  intros Gamma x U t v T Ht He.
+  generalize dependent T.
+  generalize dependent U.
+  revert Gamma.
+  induction v; simpl;
+    try solve [intros; inversion He; subst;
+               eapply local_substitution_preserves_local_typing; eauto];
+    intros.
+  - intros; inversion He; subst.
+    + econstructor.
+      * eapply weakening; eauto.
+        compute; congruence.
+      * admit.
+    + inversion H; subst.
+      econstructor; eauto.
+      * eapply weakening; eauto.
+        compute; congruence.
+      * admit.
+  - intros; inversion He; subst.
+    + econstructor.
+      * eapply weakening; eauto.
+        compute; congruence.
+      * admit.
+    + inversion H; subst.
+Admitted.
+
+Theorem preservation : forall t t' T,
+  empty |- t \in T  ->
+  t --> t'  ->
+  empty |- t' \in T.
+Proof with eauto.
+  intros t t' T HT. generalize dependent t'.
+  remember empty as Gamma.
+  eapply has_type_ind' with
+    (P := fun Gamma t T _ => Gamma = empty ->  forall (t' : tm) (HE : t --> t'), Gamma |- t' \in T)
+    (P0 := fun Gamma t T _ =>  Gamma = empty ->  forall (t' : tm) (HE : t --> t'), has_local_type Gamma t' T)
+    in HT; eauto; clear; intros; subst; try discriminate;
+    try solve [inversion HE; subst; auto].
+  - (* T_App *)
+    inversion HE; subst...
+    + eapply local_substitution_preserves_typing with T2; eauto.
+      inversion h; subst; eauto.
+  - inversion HE; subst...
+    eapply global_substitution_preserves_typing with T1; eauto.
+    inversion h; eauto.
+  - inversion HE; subst...
+    + econstructor; eauto.
+    + inversion h; subst.
+      eapply delaying_preserves_local_typing; try eassumption.
+  - inversion HE; subst...
+    + econstructor; eauto.
+    + eapply global_substitution_preserves_local_typing; eauto.
+      inversion h; subst; assumption.
+  - econstructor; eauto.
 Qed.
